getting consistent with latest HOL version

tools/splat/AADL.sig
@@ -29,7 +29,10 @@ sig
   val scrape : Json.json -> decls
   val scrape_pkgs : Json.json -> decls list
 
-  val mk_aadl_defs : string -> tyEnv -> decls -> tyEnv * thm list * thm list * (string * thm) list
-  val pkgs2hol : string -> decls list -> tyEnv * thm list * thm list * (string * thm) list
+  val mk_aadl_defs 
+    : string -> tyEnv -> decls -> tyEnv * thm list * thm list * (string * thm) list
+
+  val pkgs2hol 
+    : string -> decls list -> tyEnv * thm list * thm list * (string * thm) list
 
 end
